-

src/simp_loop/binders.lean
@@ -1,160 +1,106 @@
 /-
-Copyright (c) 2017 Johannes Hölzl. All rights reserved.
+Copyright (c) 2018 Johannes Hölzl. All rights reserved.
 Released under Apache 2.0 license as described in the file LICENSE.
 Authors: Johannes Hölzl
 
 Binder elimination
--/
-import order tactic.converter.old_conv
-
-namespace old_conv
-open tactic monad
-
-meta instance : monad_fail old_conv :=
-{ fail := λ α s, (λr e, tactic.fail (to_fmt s) : old_conv α), ..old_conv.monad }
-
-meta instance : has_monad_lift tactic old_conv :=
-⟨λα, lift_tactic⟩
-
-meta instance (α : Type) : has_coe (tactic α) (old_conv α) :=
-⟨monad_lift⟩
-
-meta def current_relation : old_conv name := λr lhs, return ⟨r, lhs, none⟩
-
-meta def head_beta : old_conv unit :=
-λ r e, do n ← tactic.head_beta e, return ⟨(), n, none⟩
-
-/- congr should forward data! -/
-meta def congr_arg : old_conv unit → old_conv unit := congr_core (return ())
-meta def congr_fun : old_conv unit → old_conv unit := λc, congr_core c (return ())
-
-meta def congr_rule (congr : expr) (cs : list (list expr → old_conv unit)) : old_conv unit := λr lhs, do
-  meta_rhs ← infer_type lhs >>= mk_meta_var, -- is maybe overly restricted for `heq`
-  t ← mk_app r [lhs, meta_rhs],
-  ((), meta_pr) ← solve_aux t (do
-    apply congr,
-    focus $ cs.map $ λc, (do
-      xs ← intros,
-      conversion (head_beta >> c xs)),
-    done),
-  rhs ← instantiate_mvars meta_rhs,
-  pr ← instantiate_mvars meta_pr,
-  return ⟨(), rhs, some pr⟩
-
-meta def congr_binder (congr : name) (cs : expr → old_conv unit) : old_conv unit := do
-  e ← mk_const congr,
-  congr_rule e [λbs, do [b] ← return bs, cs b]
-
-meta def funext' : (expr → old_conv unit) → old_conv unit := congr_binder ``_root_.funext
-
-meta def propext' {α : Type} (c : old_conv α) : old_conv α := λr lhs, (do
-  guard (r = `iff),
-  c r lhs)
-<|> (do
-  guard (r = `eq),
-  ⟨res, rhs, pr⟩ ← c `iff lhs,
-  match pr with
-  | some pr := return ⟨res, rhs, (expr.const `propext [] : expr) lhs rhs pr⟩
-  | none := return ⟨res, rhs, none⟩
-  end)
-
-meta def apply (pr : expr) : old_conv unit :=
-λ r e, do
-  sl ← simp_lemmas.mk.add pr,
-  apply_lemmas sl r e
-
-meta def applyc (n : name) : old_conv unit :=
-λ r e, do
-  sl ← simp_lemmas.mk.add_simp n,
-  apply_lemmas sl r e
-
-meta def apply' (n : name) : old_conv unit := do
-  e ← mk_const n,
-  congr_rule e []
-
-end old_conv
-
-open expr tactic old_conv
-
-/- Binder elimination:
 
 We assume a binder `B : p → Π (α : Sort u), (α → t) → t`, where `t` is a type depending on `p`.
 Examples:
   ∃: there is no `p` and `t` is `Prop`.
   ⨅, ⨆: here p is `β` and `[complete_lattice β]`, `p` is `β`
 
-Problem: ∀x, _ should be a binder, but is not a constant!
+Problem: ∀x, _ should be a binder, but is not a constant! Needs special matcher.
 
 Provide a mechanism to rewrite:
 
   B (x : α) ..x.. (h : x = t), p x  =  B ..x/t.., p t
 
 Here ..x.. are binders, maybe also some constants which provide commutativity rules with `B`.
-
 -/
+import simp_loop.conv
+
+namespace simp_loop
+open conv_t tactic expr
 
 meta structure binder_eq_elim :=
-(match_binder  : expr → tactic (expr × expr))            -- returns the bound type and body
-(adapt_rel     : old_conv unit → old_conv unit)          -- optionally adapt `eq` to `iff`
-(apply_comm    : old_conv unit)                          -- apply commutativity rule
-(apply_congr   : (expr → old_conv unit) → old_conv unit) -- apply congruence rule
-(apply_elim_eq : old_conv unit)                          -- (B (x : β) (h : x = t), s x) = s t
+(match_binder  : expr → tactic (expr × expr))    -- returns the bound type and body
+(adapt_rel     : conv unit → conv unit)          -- optionally adapt `eq` to `iff`
+(apply_comm    : conv unit)                      -- apply commutativity rule
+(apply_congr   : (expr → conv unit) → conv unit) -- apply congruence rule
+(apply_elim_eq : conv unit)                      -- (B (x : β) (h : x = t), s x) = s t
 
-meta def binder_eq_elim.check_eq (b : binder_eq_elim) (x : expr) : expr → tactic unit
+namespace binder_eq_elim
+
+protected meta def check_eq (b : binder_eq_elim) (x : expr) : expr → tactic unit
 | `(@eq %%β %%l %%r) := guard ((l = x ∧ ¬ x.occurs r) ∨ (r = x ∧ ¬ x.occurs l))
 | _ := fail "no match"
 
-meta def binder_eq_elim.pull (b : binder_eq_elim) (x : expr) : old_conv unit := do
-  (β, f) ← lhs >>= (lift_tactic ∘ b.match_binder),
-  guard (¬ x.occurs β)
-  <|> b.check_eq x β
-  <|> (do
-    b.apply_congr $ λx, binder_eq_elim.pull,
-    b.apply_comm)
+protected meta def push (b : binder_eq_elim) (x : expr) : ℕ → conv unit
+| 0       := do trace "finished push", trace_lhs,
+  return ()
+| (n + 1) :=
+  (do trace ("push " ++ to_string n ++ " the current binder to the right"), trace_lhs,
+    b.apply_comm,
+    b.apply_congr $ λx, push n) <|>
+  (do trace ("push " ++ to_string n ++ " there is a dependency: switch to the right binder"), trace_lhs,
+    b.apply_congr $ λx, push n)
 
-meta def binder_eq_elim.push (b : binder_eq_elim) : old_conv unit :=
+protected meta def pull (b : binder_eq_elim) : ℕ → conv unit
+ | 0       := do trace "finished pull", trace_lhs,
   b.apply_elim_eq
-<|> (do
-  b.apply_comm,
-  b.apply_congr $ λx, binder_eq_elim.push)
-<|> (do
-  b.apply_congr $ b.pull,
-  binder_eq_elim.push)
+| (n + 1) :=
+  (do trace ("pull (" ++ to_string n ++ ") the non-dependent binders to the left"), trace_lhs,
+    b.apply_comm,
+    b.apply_congr $ λx, pull n) <|>
+  (do trace ("pull (" ++ to_string n ++ ") the right (dependent binder) to the right, then try again"), trace_lhs,
+    b.apply_congr $ λe, b.push e (n + 1),
+    pull n)
 
-meta def binder_eq_elim.check (b : binder_eq_elim) (x : expr) : expr → tactic unit
-| e := do
+protected meta def check (b : binder_eq_elim) (x : expr) : ℕ → expr → tactic ℕ
+| i e := do
   (β, f) ← b.match_binder e,
-  b.check_eq x β
+  (b.check_eq x β >> return i)
   <|> (do
     (lam n bi d bd) ← return f,
     x ← mk_local' n bi d,
-    binder_eq_elim.check $ bd.instantiate_var x)
+    check (i + 1) (bd.instantiate_var x))
 
-meta def binder_eq_elim.old_conv (b : binder_eq_elim) : old_conv unit := do
+protected meta def conv (b : binder_eq_elim) : conv unit := do
   (β, f) ← lhs >>= (lift_tactic ∘ b.match_binder),
   (lam n bi d bd) ← return f,
   x ← mk_local' n bi d,
-  b.check x (bd.instantiate_var x),
-  b.adapt_rel b.push
+  i ← b.check x 0 (bd.instantiate_var x),
+  b.adapt_rel (b.pull i)
+
+
+
+end binder_eq_elim
+
+section exists_eq_elim
 
 theorem {u v} exists_comm {α : Sort u} {β : Sort v} (p : α → β → Prop) :
   (∃a b, p a b) ↔ (∃b a, p a b) :=
 ⟨λ⟨a, ⟨b, h⟩⟩, ⟨b, ⟨a, h⟩⟩, λ⟨a, ⟨b, h⟩⟩, ⟨b, ⟨a, h⟩⟩⟩
 
 theorem {u v} exists_elim_eq_left {α : Sort u} (a : α) (p : Π(a':α), a' = a → Prop) :
-  (∃(a':α)(h : a' = a), p a' h) ↔ p a rfl :=
+  (∃(a':α) (h : a' = a), p a' h) ↔ p a rfl :=
 ⟨λ⟨a', ⟨h, p_h⟩⟩, match a', h, p_h with ._, rfl, h := h end, λh, ⟨a, rfl, h⟩⟩
 
 theorem {u v} exists_elim_eq_right {α : Sort u} (a : α) (p : Π(a':α), a = a' → Prop) :
-  (∃(a':α)(h : a = a'), p a' h) ↔ p a rfl :=
+  (∃(a':α) (h : a = a'), p a' h) ↔ p a rfl :=
 ⟨λ⟨a', ⟨h, p_h⟩⟩, match a', h, p_h with ._, rfl, h := h end, λh, ⟨a, rfl, h⟩⟩
 
 meta def exists_eq_elim : binder_eq_elim :=
 { match_binder  := λe, (do `(@Exists %%β %%f) ← return e, return (β, f)),
-  adapt_rel     := propext',
-  apply_comm    := applyc ``exists_comm,
-  apply_congr   := congr_binder ``exists_congr,
-  apply_elim_eq := apply' ``exists_elim_eq_left <|> apply' ``exists_elim_eq_right }
+  adapt_rel     := propext,
+  apply_comm    := apply_const ``exists_comm,
+  apply_congr   := congr_binder `exists_congr,
+  apply_elim_eq := apply_const ``exists_elim_eq_left <|> apply_const ``exists_elim_eq_right }
+
+end exists_eq_elim
+
+section forall_eq_elim
 
 theorem {u v} forall_comm {α : Sort u} {β : Sort v} (p : α → β → Prop) :
   (∀a b, p a b) ↔ (∀b a, p a b) :=
@@ -170,10 +116,48 @@ theorem {u v} forall_elim_eq_right {α : Sort u} (a : α) (p : Π(a':α), a = a'
 
 meta def forall_eq_elim : binder_eq_elim :=
 { match_binder  := λe, (do (expr.pi n bi d bd) ← return e, return (d, expr.lam n bi d bd)),
-  adapt_rel     := propext',
-  apply_comm    := applyc ``forall_comm,
-  apply_congr   := congr_binder ``forall_congr,
-  apply_elim_eq := apply' ``forall_elim_eq_left <|> apply' ``forall_elim_eq_right }
+  adapt_rel     := propext,
+  apply_comm    := apply_const ``forall_comm,
+  apply_congr   := congr_binder `forall_congr,
+  apply_elim_eq := apply_const ``forall_elim_eq_left <|> apply_const ``forall_elim_eq_right }
+
+end forall_eq_elim
+
+section test
+
+universes u v w w₂
+variables {α : Type u} {β : Type v} {ι : Sort w} {ι₂ : Sort w₂} {a : α} {γ : β → Type} {δ : α → Type}
+  {f : α → β} {p : β → Prop}
+
+example : (∃b, ∃c:γ b, ∃h : f a = b, p b) ↔ (∃c:γ (f a), p (f a)) :=
+by conversion exists_eq_elim.conv
+
+example : (∃b, ∃c:γ b, ∃a, ∃h : f a = b, p b) ↔ (∃a, ∃c:γ (f a), p (f a)) :=
+by conversion exists_eq_elim.conv
+
+example {f : Πa, δ a → β} :
+  (∃b, ∃c:γ b, ∃a, ∃d:δ a, ∃h : f a d = b, p b) ↔ (∃a, ∃d:δ a, ∃c:γ (f a d), p (f a d)) :=
+by conversion exists_eq_elim.conv
+
+example {f : Πa, δ a → β} :
+  (∃b, ∃a, ∃c:γ b, ∃d:δ a, ∃h : f a d = b, p b) ↔ (∃a, ∃d:δ a, ∃c:γ (f a d), p (f a d)) :=
+by conversion exists_eq_elim.conv
+
+example {f : Πa, δ a → β} :
+  (∃b, ∃a, ∃d:δ a, ∃c:γ b, ∃h : f a d = b, p b) ↔ (∃a, ∃d:δ a, ∃c:γ (f a d), p (f a d)) :=
+by conversion exists_eq_elim.conv
+
+example {f : Πa, δ a → β} :
+  (∃b, ∃a, ∃d:δ a, ∃h : f a d = b, ∃c:γ b, p b) ↔ (∃a, ∃d:δ a, ∃c:γ (f a d), p (f a d)) :=
+by conversion exists_eq_elim.conv
+
+example {f : Πa, δ a → β} :
+  (∃b, ∃a, ∃d:δ a, ∃h' : a = a ∧ b = b, ∃h : f a d = b, ∃c:γ b, p b) ↔ _ :=
+by conversion exists_eq_elim.conv
+
+end test
+
+#exit -- lattice theory only in mathlib
 
 meta def supr_eq_elim : binder_eq_elim :=
 { match_binder  := λe, (do `(@lattice.supr %%α %%β %%cl %%f) ← return e, return (β, f)),
@@ -189,12 +173,6 @@ meta def infi_eq_elim : binder_eq_elim :=
   apply_congr   := congr_arg ∘ funext',
   apply_elim_eq := applyc ``lattice.infi_infi_eq_left <|> applyc ``lattice.infi_infi_eq_right }
 
-
-universes u v w w₂
-variables {α : Type u} {β : Type v} {ι : Sort w} {ι₂ : Sort w₂} {s t : set α} {a : α}
-
-@[simp] theorem mem_image {f : α → β} {b : β} : b ∈ set.image f s = ∃a, a ∈ s ∧ f a = b := rfl
-
 section
 open lattice
 variables [complete_lattice α]
@@ -202,13 +180,13 @@ variables [complete_lattice α]
 theorem Inf_image {s : set β} {f : β → α} : Inf (set.image f s) = (⨅ a ∈ s, f a) :=
 begin
   simp [Inf_eq_infi, infi_and],
-  conversion infi_eq_elim.old_conv,
+  conversion infi_eq_elim.conv,
 end
 
 theorem Sup_image {s : set β} {f : β → α} : Sup (set.image f s) = (⨆ a ∈ s, f a) :=
 begin
   simp [Sup_eq_supr, supr_and],
-  conversion supr_eq_elim.old_conv,
+  conversion supr_eq_elim.conv,
 end
 
 end
